---
title: Hatcher Exercise 3.1.5
layout: math-page
chapter: 3
exercise: 1.5
---


Let $$\varphi$$ be a 1-cochain in $$X$$ with coefficients in $$G$$ -- i.e. $$\varphi \in C^1(X,G) = \Hom(C_1(X), G)$$.
$$\varphi$$ is a function from 1-chains in $$X$$ to $$G$$.
Since, in general, singular 1-chains are precisely paths in $$X$$, we will consider $$\varphi$$ as a function from paths in $$X$$ to $$G$$.
For paths $$f$$ and $$g$$, we will use $$f \cdot g$$ to refer to path concatenation (not to be confused with the group operation in $$C_1(X)$$).

For all of the following, assume $$\varphi$$ is a co-cycle -- i.e. $$\varphi \in \ker \delta_1$$, where $$\delta_1 : C^1(X,G) \rightarrow C^2(X,G)$$ is the coboundary map.

**Theorem**:
$$\varphi(f \cdot g) = \varphi(f) + \varphi(g)$$.

---

*Proof*:
Consider a singular two chain $$F$$ -- that is, a map from the 2-simplex $$[abc]$$ to $$X$$ -- such that $$F \vert_{[a b]} = f$$ and $$F \vert_{[b c]} = g$$.
We then have that $$F \vert_{[ac]}$$ is homotopic to $$f \cdot g$$.
To see this, just consider that there is a deformation retraction of the simplex $$[abc]$$ to the edge $$[ac]$$ (by simply crushing it) -- compose this deformation retraction with $$F$$ to get a homotopy from the image of $$F \vert_{[ab] \cdot [bc]}$$ which is $$f \cdot g$$ to the image of $$F \vert_{[ac]}$$.
Now, since $$\varphi$$ is a cocycle, $$\delta_1 \varphi$$ is the zero map and $$(\delta_1 \varphi)(F) = 0$$.
Then,

$$
\begin{align*}
& (\delta_1 \varphi)(F) = \varphi(F \vert_{[bc]}) - \varphi(F \vert_{[ac]}) + \varphi(F_{[ab]}) = 0 \\
\Rightarrow \enspace & \varphi(g) - \varphi(f \cdot g) + \varphi(f) = 0 \\
\Rightarrow \enspace & \varphi(f \cdot g) = \varphi(f) + \varphi(g)
\end{align*}
$$

$$\mjqed$$

**Corollary**:
$$\varphi$$ is zero on constant paths.

---

*Proof*:
If $$f$$ is a constant path, then $$f \cdot f = f$$.
By the last theorem, $$\varphi(f \cdot f) = \varphi(f) = \varphi(f) + \varphi(f)$$, which could only be true in the group $$G$$ if $$\varphi(f) = 0$$.

$$\mjqed$$

---

**Theorem**:
If $$f$$ is homotopic to $$g$$ (fixing endpoints), then $$\varphi(f) = \varphi(g)$$

---

*Proof*:
Let $$a = (0, 0), b = (0, 1), c= (1,1)$$ in $$\mathbb{R}^2$$ explicitly describe the vertices of a 2-simplex.
We will explicitly describe two singular 2-chains $$F, G : [abc] \rightarrow X$$.
Let $$H : I \times I \rightarrow X$$ be the homotopy from $$f$$ to $$g$$, so that $$H(0, \cdot) = f$$ and $$H(1, \cdot) = g$$.

Let $$F(x,y) = H(y,x)$$.
Observe that $$F\vert_{[ab]} = f$$ and $$F\vert_{[bc]} = f(1) = g(1)$$ (the constant path).
Then $$F\vert_{[ac]} = z$$, where $$z$$ is the path $$t \mapsto H(t,t)$$.
Let $$G(x,y) = H(x,y)$$.
Then, $$G\vert_{[ab]} = f(0) = g(0)$$ (the constant path) and $$G\vert_{[bc]} = g$$.
In particular, $$G\vert_{[ac]} = z$$ again.
Then, we have:

$$
(\delta_1 \varphi)(F) = \varphi(f) - \varphi(z) + \varphi(f(1)) = 0
$$

But since $$\varphi$$ is zero on constant paths, the last term is zero and we have $$\varphi(f) = \varphi(z)$$.
Applying the same argument to $$G$$ gives $$\varphi(g) = \varphi(z)$$, and we have $$\varphi(f) = \varphi(g)$$ by transitivity.

$$\mjqed$$

---

**Theorem**:
$$\varphi$$ is a coboundary if and only if $$\varphi(f)$$ depends only on the endpoints of $$f$$

---

*Proof*:
Let $$f : [ab] \rightarrow X$$ be an arbitrary singular 1-chain.
If $$\varphi$$ is a coboundary, then $$\varphi = \delta_0 \gamma$$ for a 0-cochain $$\gamma$$.
But then $$\varphi(f) = \gamma(f\vert_{[b]}) - \gamma(f\vert_{[a]})$$, so $$\varphi$$ only depends on the endpoints.

Suppose that $$\varphi(f)$$ depends only on the endpoints of $$f$$ for any $$f$$.
Pick a basepoint $$x_0 \in X$$ and define a 0-cochain $$\gamma$$ by $$\gamma(x) = \varphi(f_x)$$ where $$f_x$$ is any path from $$x_0$$ to $$x$$.
This is well-defined due to the supposition about $$\varphi$$.
Then, for any path $$g$$ from $$a$$ to $$b$$,
pick some path $$f_a$$ from $$x_0$$ to $$a$$, and notice that $$f_a \cdot g$$ is some path from $$x_0$$ to $$b$$.
Then, we have:

$$
(\delta_0 \gamma)(g) = \gamma(b) - \gamma(a) = \varphi(f_a \cdot g) - \varphi(f_a) = \varphi(f_a) + \varphi(g) - \varphi(f_a) = \varphi(g)
$$

using the first theorem.
Thus, $$\delta_0 \gamma = \varphi$$.

$$\mjqed$$
