---
title: Hatcher Exercise 3.1.6
layout: math-page
chapter: 3
exercise: 1.6
order: 106
description: Computing co-homology of basic cell complexes
---



We compute the simplicial cohomology of some basic cell complexes directly from the definitions, using coefficients in both $$\mathbb{Z}$$ and $$\mathbb{Z}^2$$.

---

**(a)**
Let $$X = T^2$$, with the cell complex structure given in Hatcher section 2.1.
First work with coefficients in $$\mathbb{Z}$$.
The cochain complex is:

$$
0 \leftarrow \Delta^2 \xleftarrow{\delta_1} \Delta^1 \xleftarrow{\delta_0} \Delta^0 \leftarrow 0
$$

Specifically,

$$
0 \leftarrow \la U^*, L^* \ra \xleftarrow{\delta_1} \la a^*,b^*,c^* \ra \xleftarrow{\delta_0} \la v^* \ra \leftarrow 0
$$

where we are viewing, for example $$a^*$$, as the map assigning $$1$$ to the edge $$a$$ and $$0$$ to the other edges.
Clearly then, the group $$\Delta^1$$ is generated by $$a^*$$, $$b^*$$, and $$c^*$$ (similarly for the others).

We have $$(\delta_0 v^*)(e) = v^*(v) - v^*(v)$$ for all edges $$e$$, so $$\delta_0 = 0$$.
For $$\delta_1$$, we have $$(\delta_1 a^*)(U) = a^*(a) + a^*(b) - a^*(c) = 1$$, and $$(\delta_1 a^*)(L) = a^*(c) - a^*(a) - a^*(b) = -1$$.
Then, we can express $$\delta_1 a^*$$ as $$\delta_1 a^* = U^* - L^*$$.
Similarly, we find $$\delta_1 b^* = U^* - L^*$$ and $$\delta_1 c^* = L^* - U^*$$.
To summarize,

$$
\delta_0 = \left( \begin{array}{c}
0 \\
0 \\
0
\end{array} \right)
\xrightarrow{SNF}
\left( \begin{array}{c}
0 \\
0 \\
0
\end{array} \right)
\qquad
\delta_1 = \left( \begin{array}{ccc}
1 & 1 & -1 \\
-1 & -1 & 1
\end{array} \right)
\xrightarrow{SNF}
\left( \begin{array}{ccc}
1 & 0 & 0 \\
0 & 0 & 0
\end{array} \right)
$$

Determining the homology of the cochain complex is now a matter of algebra determined completely from the matrices (keeping in mind the homology groups are $$\ker \delta_n / \im \delta_{n-1}$$, instead of $$\im \delta_{n+1}$$), and we find:

$$
H^0 = \mathbb{Z} \qquad H^1 = \mathbb{Z}^2 \qquad H^2 = \mathbb{Z}
$$

Of course, this matches the homology of the torus exactly, because there is no torsion.

If we work with coefficients in $$\mathbb{Z}_2$$, the maps change slightly.
We still have $$\delta_0 = 0$$, but $$\delta_1(a^*) = \delta_1(b^*) = \delta_1(c^*) = U^* + L^*$$.
Then we have

$$
\delta_1 = \left( \begin{array}{ccc}
1 & 1 & 1 \\
1 & 1 & 1
\end{array} \right)
\xrightarrow{SNF}
\left( \begin{array}{ccc}
1 & 0 & 0 \\
0 & 0 & 0
\end{array} \right)
$$

and the homology is:

$$
H^0 = \mathbb{Z}_2 \qquad H^1 = \mathbb{Z}_2^2 \qquad H^2 = \mathbb{Z}_2
$$

---

**(b)**
Let $$X = \mathbb{R}P^2$$, with the cell complex structure from Hatcher 2.1.
First work with coefficients in $$\mathbb{Z}$$.
The cochain complex is:

$$
0 \leftarrow \la U^*, L^* \ra \xleftarrow{\delta_1} \la a^*, b^*, c^* \ra \xleftarrow{\delta_0} \la v^*, w^* \ra \leftarrow 0
$$

We have $$(\delta_0 v^*)(a) = v^*(w) - v^*(v) = -1$$, and likewise $$(\delta_0 v^*)(b) = -1$$.
Also $$(\delta_0 v^*)(c) = v^*(v) - v^*(v) = 0$$.
So $$\delta_0 v^* = -(a^* + b^*)$$.
Similarly we find $$\delta_0 w^* = a^* + b^*$$.
For $$\delta_1$$, we have $$(\delta_1 a^*)(U) = a^*(a) - a^*(b) - a^*(c) = 1$$ and $$(\delta_1 a^*)(L) = a^*(c) + a^*(a) - a^*(b) = -1$$.
Thus $$\delta_1 a^* = U^* - L^*$$.
Similarly we find $$\delta_1 b^* = -(U^* + L^*)$$ and $$\delta_1 c^* = -U^* + L^*$$.
Summarizing:

$$
\delta_0 = \left( \begin{array}{cc}
-1 & 1 \\
-1 & 1 \\
0 & 0
\end{array} \right)
\xrightarrow{SNF}
\left( \begin{array}{cc}
1 & 0 \\
0 & 0 \\
0 & 0
\end{array} \right)
\qquad
\delta_1 = \left( \begin{array}{ccc}
1 & -1 & -1 \\
-1 & -1 & 1
\end{array} \right)
\xrightarrow{SNF}
\left( \begin{array}{ccc}
1 & 0 & 0 \\
0 & 2 & 0
\end{array} \right)
$$

and we arrive at:

$$
H^0 = \mathbb{Z} \qquad H^1 = 0 \qquad H^2 = \mathbb{Z}_2
$$

If we work with coefficients in $$\mathbb{Z}^2$$, the maps change as follows:

$$
\delta_0 = \left( \begin{array}{cc}
1 & 1 \\
1 & 1 \\
0 & 0
\end{array} \right)
\xrightarrow{SNF}
\left( \begin{array}{cc}
1 & 0 \\
0 & 0 \\
0 & 0
\end{array} \right)
\qquad
\delta_1 = \left( \begin{array}{ccc}
1 & 1 & 1 \\
1 & 1 & 1
\end{array} \right)
\xrightarrow{SNF}
\left( \begin{array}{ccc}
1 & 0 & 0 \\
0 & 0 & 0
\end{array} \right)
$$

and we arrive at:

$$
H^0 = \mathbb{Z}_2 \qquad H^1 = \mathbb{Z}_2 \qquad H^2 = \mathbb{Z}_2
$$

---

**(c)**
Finally, let $$X = K^2$$ with the cell structure from 2.1.
Again, work with $$\mathbb{Z}$$ coefficients first.
The cochain complex is:

$$
0 \leftarrow \la U^*, L^* \ra \xleftarrow{\delta_1} \la a^*,b^*,c^* \ra \xleftarrow{\delta_0} \la v^* \ra \leftarrow 0
$$

We have $$\delta_0 = 0$$, because there is only one vertex (reasoning as in part (a)).
We have $$(\delta_1 a^*)(U) = a^*(a) + a^*(b) - a^*(c) = 1$$, and $$(\delta_1 a^*)(L) = a^*(c) + a^*(a) - a^*(b) = 1$$.
So we find $$\delta_1 a^* = U^* + L^*$$.
For the others, we find $$\delta_1 b^* = U^* - L^*$$ and $$\delta_1 c^* = -U^* + L^*$$.
So the maps are:

$$
\delta_0 = \left( \begin{array}{c}
0 \\
0 \\
0
\end{array} \right)
\xrightarrow{SNF}
\left( \begin{array}{c}
0 \\
0 \\
0
\end{array} \right)
\qquad
\delta_1 = \left( \begin{array}{ccc}
1 & 1 & -1 \\
1 & -1 & 1
\end{array} \right)
\xrightarrow{SNF}
\left( \begin{array}{ccc}
1 & 0 & 0 \\
0 & 2 & 0
\end{array} \right)
$$

and we have:

$$
H^0 = \mathbb{Z} \qquad H^1 = \mathbb{Z} \qquad H^2 = \mathbb{Z}_2
$$

If we work with coefficients in $$\mathbb{Z}_2$$, $$\delta_1$$ changes as follows:

$$
\delta_1 = \left( \begin{array}{ccc}
1 & 1 & 1 \\
1 & 1 & 1
\end{array} \right)
\xrightarrow{SNF}
\left( \begin{array}{ccc}
1 & 0 & 0 \\
0 & 0 & 0
\end{array} \right)
$$

and we arrive at:

$$
H^0 = \mathbb{Z}_2 \qquad H^1 = \mathbb{Z}_2^2 \qquad H^2 = \mathbb{Z}_2
$$
