---
title: Exercise 1.3.27
chapter: 1
exercise: 3.27
order: 327
layout: math-page
description: The functor categories $$[\mathbf{A}^{\text{op}}, \mathbf{B}^{\text{op}}]$$ and $$[\mathbf{A}, \mathbf{B}]^{\text{op}}$$ are isomorphic
---

$$\newcommand\cx{[\mathbf{A}^{op}, \mathbf{B}^{op}]}$$
$$\newcommand\cy{[\mathbf{A}, \mathbf{B}]^{op}}$$

**Theorem**:
For categories $$\mathbf{A}$$ and $$\mathbf{B}$$, $$\cx$$ is isomorphic to $$\cy$$.


*Proof*:
We'll first need to define a functor $$\mathcal{F} : \cx \rightarrow \cy$$.
Let $$F$$ be an object of $$\cx$$ -- that is a functor $$\mathbf{A}^{op} \rightarrow \mathbf{B}^{op}$$.
Then, let $$\mathcal{F}(F)$$ be a functor $$\mathbf{A} \rightarrow \mathbf{B}$$ such that for an object $$A \in \mathbf{A}$$, $$\mathcal{F}(F)(A) = F(A)$$, and for an arrow $$f$$ of $$\mathbf{A}$$, $$\mathcal{F}(F)(f) = F(f^{op})^{op}$$ (flip the arrow, send it through $$F$$, and flip it again).

Now, having described what $$\mathcal{F}$$ does to objects in $$\cx$$ (functors), we need to describe what $$\mathcal{F}$$ does to arrows (natural transformations).
If $$\alpha : F \rightarrow G$$ is a natural transformation between $$F, G  : \mathbf{A}^{op} \rightarrow \mathbf{B}^{op}$$,
We need $$\mathcal{F}(\alpha)$$ to be natural transformation $$\mathcal{F}(G) \rightarrow \mathcal{F}(F)$$ between $$\mathcal{F}(G), \mathcal{F}(F) : \mathbf{A} \rightarrow \mathbf{B}$$.
For $$A \in \mathbf{A}$$, notice that $$\alpha_A$$ is an arrow in $$\mathbf{B}^{op}$$ whose domain is $$F(A)$$ and whose codomain is $$G(A)$$.
So we can just define $$\mathcal{F}(\alpha)_A = (\alpha_A)^{op}$$, which is an arrow in $$\mathbf{B}$$ whose domain is $$G(A) = \mathcal{F}(G)(A)$$ and whose codomain is $$F(A) = \mathcal{F}(F)(A)$$.
Then, we have a well-defined map $$\mathcal{F}(\alpha)_A : \mathcal{F}(G)(A) \rightarrow \mathcal{F}(F)(A)$$ for each $$A$$, and $$\mathcal{F}(\alpha)$$ is a natural transformation as prescribed.

We quickly verify that $$\mathcal{F}$$ is indeed a functor.
If $$1_F$$ is the identity natural transformation on $$F \in \cx$$, then

$$
\mathcal{F}(1_F)_A = ((1_F)_A)^{op} = (1_{F(A)})^{op} = 1_{F(A)} = 1_{\mathcal{F}(F)(A)} = (1_{\mathcal{F}(F)})_A
$$

so $$\mathcal{F}(1_F) = 1_{\mathcal{F}(F)}$$.

Suppose $$F \xrightarrow{\alpha} G \xrightarrow{\beta} H$$ are natural transformations.
Then we have

$$
\mathcal{F}(\beta \alpha)_A = ((\beta \alpha)_A)^{op} = (\beta_A \alpha_A)^{op} = (\alpha_A)^{op} (\beta_A)^{op} = \mathcal{F}(\alpha)_A \mathcal{F}(\beta)_A
$$

(composed in the opposite order because $$\mathcal{F}$$ is contravariant).

One can obtain the inverse functor by applying the identical construction starting with $$\mathcal{A}^{op}$$ and $$\mathcal{B}^{op}$$.
In this way, we get a functor $$\mathcal{G} : [\mathbf{A}, \mathbf{B}] \rightarrow [\mathbf{A}^{op}, \mathbf{B}^{op}]^{op}$$.
But, this can equally well be described as a functor $$\mathcal{G} : \cy \rightarrow \cx$$.
Either way, $$\mathcal{G}$$ is defined by identical rules to $$\mathcal{F}$$.
If $$F \in \cx$$, recall $$\mathcal{F}(F)(A) = F(A)$$ and $$\mathcal{F}(F)(f) = F(f^{op})^{op}$$.
So, $$\mathcal{G}(\mathcal{F}(F))(A) = \mathcal{F}(F)(A) = F(A)$$ and $$\mathcal{G}(\mathcal{F}(F))(f) = (\mathcal{F}(F)(f^{op}))^{op} = (F(f)^{op})^{op} = F(f)$$.
So, $$(\mathcal{G} \circ \mathcal{F})(F) = F$$.
If $$\alpha : F \rightarrow G$$ is a natural transformation, recall that we have $$\mathcal{F}(\alpha)_A = (\alpha_A)^{op}$$.
So, $$\mathcal{G}(\mathcal{F}(\alpha))_A = (\mathcal{F}(\alpha)_A)^{op} = ((\alpha_A)^{op})^{op} = \alpha_A$$.
So $$(\mathcal{G} \circ \mathcal{F})(\alpha) = \alpha$$.
Together, this means that $$\mathcal{G} \circ \mathcal{F}$$ is the identity functor on $$\cx$$.
It follows symmetrically that $$\mathcal{F} \circ \mathcal{G}$$ is the identity on $$\cy$$.
Thus, $$\cx$$ and $$\cy$$ are isomorphic.
